src/lib/GPU.HReduce_U64_Plus.fsti
@@ -1,0 +1,92 @@
+module GPU.HReduce_U64_Plus
+
+(* This module is specialized to U64 and addition.
+
+The only admits are a boring fact about associativity of add_mod (unsure why
+it's not already trivial in F* ) and lack of overflow of the iteration counter.
+This last thing should fall out from the fact that any the size of an array must
+fit in a sizet, and the log of that size even more so. *)
+
+#lang-pulse
+
+open GPU
+open GPU.Barrier.RPM
+open GPU.Math
+open GPU.Seq.Common
+
+module A = Pulse.Lib.Array
+module SZ = FStar.SizeT
+module U32 = FStar.UInt32
+module U64 = FStar.UInt64
+
+let size : sz = 1024sz
+
+(* no polymorphism, but at least keep the definitions here *)
+let ety = u64
+inline_for_extraction noextract let op = U64.add_mod
+inline_for_extraction noextract let neu = 0uL
+
+(* using seq_fold_left op neu directly in pulse code blows up
+in many colorful ways. Probably the refinment of op? Anyway, 
+specialize it here. *)
+let sum (s : seq ety) : GTot ety =
+  seq_fold_left op neu s
+  
+(* Ownership of array r between i and j. The first value of that slice
+is the reduction of all the values in the (original) slice v. *)
+let gpu_pts_to_slice_sum_inner
+  (#sz:nat)
+  (r : gpu_array u64 sz)
+  (i j :nat)
+  (v : seq u64)
+  (s : seq u64)
+: slprop
+= gpu_pts_to_array_slice r i j s
+  ** pure (i < j /\ j <= sz /\
+           Seq.length v = sz /\
+           Seq.length s = j - i /\
+           Seq.index s 0 = sum (Seq.slice v i j))
+
+let gpu_pts_to_slice_sum
+  (#sz:nat)
+  ([@@@equate_strict] r: gpu_array u64 sz)
+  (i j:nat)
+  (v: seq u64)
+: slprop
+= if_ (i < j && j <= sz) (exists* s. gpu_pts_to_slice_sum_inner #sz r i j v s)
+
+// Barrier
+
+val barrier_matrix (nth: nat) (r : gpu_array u64 nth) (v: seq u64) (it from to: nat): slprop
+
+[@@pulse_unfold]
+let kpre (nth: nat) (a : gpu_array u64 nth) (s : erased (seq u64))
+  (#_: squash (Seq.length s == nth)) (tid:nat{tid < nth})
+  : slprop =
+    gpu_pts_to_array_slice a tid (tid+1) seq![Seq.index s tid]
+
+[@@pulse_unfold]
+let kpost (nth: nat) (a : gpu_array u64 nth) (s : erased (seq u64))
+  (#_: squash (Seq.length s == nth)) (tid:nat{tid < nth})
+  : slprop =
+    if_ (tid = 0) (gpu_pts_to_slice_sum a 0 nth s)
+
+[@@ CPrologue "__device__"]
+inline_for_extraction
+fn kernel
+  (nth : sz { 0 < SZ.v nth /\ SZ.v nth <= 1024 })
+  (a : gpu_array u64 nth)
+  (#s :  erased (seq u64))
+  (#_: squash (Seq.length s == nth))
+  (etid : erased tid_t { (gdim_x etid <: nat) == 1ul /\ (bdim_x etid <: nat) == SZ.sizet_to_uint32 nth })
+  requires
+    gpu **
+    thread_id etid **
+    mbarrier_tok nth (barrier_matrix nth a s) 0 (tidx_x etid) **
+    kpre nth a s (thread_index etid)
+  ensures 
+    gpu **
+    thread_id etid **
+    (exists* it. mbarrier_tok nth (barrier_matrix nth a s) it (tidx_x etid)) **
+    kpost nth a s (thread_index etid)
+
